aes-256

code/aes/Hacl.Impl.Aes128.NI.fst
@@ -14,14 +14,17 @@ noextract inline_for_extraction let nb =  4
 noextract inline_for_extraction let nk =  4 // 4, 6, or 8 for 128/192/256
 noextract inline_for_extraction let nr =  10 // 10, 12, or 14 for 128/192/256
 
-type block = lbytes 16
-type skey  = lbytes 16
-type skey256  = lbytes 32
+noextract inline_for_extraction let blocklen =  16 // 4 * nb
+noextract inline_for_extraction let keylen   =  16 // 4 * nk
+noextract inline_for_extraction let xkeylen  =  176 // 4 * nb * (nr + 1)
+
+type block = lbytes blocklen
+type skey  = lbytes keylen
 
 type state = lbuffer vec128 4
 type key1 =  lbuffer vec128 1
 type keyr =  lbuffer vec128 9
-type keyex = lbuffer vec128 15 // Saving space for AES-256
+type keyex = lbuffer vec128 11
 
 inline_for_extraction
 val aes_enc: st:state -> key:key1 -> ST unit
@@ -43,16 +46,6 @@ let aes_enc_last st key =
     st.(size 2) <- ni_aes_enc_last st.(size 2) key.(size 0);
     st.(size 3) <- ni_aes_enc_last st.(size 3) key.(size 0)
 
-let rcon =  gcreateL [u8(0x8d); u8(0x01); u8(0x02); u8(0x04); u8(0x08); u8(0x10); u8(0x20); u8(0x40); u8(0x80); u8(0x1b); u8(0x36)]
-
-inline_for_extraction
-val aes_keygen_assist: ok:key1 -> ik:key1 -> rcon:uint8 -> ST unit
-			     (requires (fun h -> live h ok /\ live h ik))
-			     (ensures (fun h0 _ h1 -> live h1 ok /\ live h1 ik /\ modifies (loc_buffer ok) h0 h1))
-let aes_keygen_assist ok ik rcon = 
-    ok.(size 0) <- ni_aes_keygen_assist ik.(size 0) rcon		      
-
-
 inline_for_extraction
 val add_round_key: st:state -> key:key1 -> ST unit
 			     (requires (fun h -> live h st /\ live h key))
@@ -63,27 +56,36 @@ let add_round_key st key =
     st.(size 2) <- vec128_xor st.(size 2) key.(size 0);
     st.(size 3) <- vec128_xor st.(size 3) key.(size 0)
 
-val enc_rounds: st:state -> key:keyr -> n:size_t -> ST unit
+val enc_rounds: st:state -> key:keyr -> ST unit
 	     (requires (fun h -> live h st /\ live h key))
 	     (ensures (fun h0 _ h1 -> live h1 st /\ live h1 key /\ modifies (loc_buffer st) h0 h1))
-let enc_rounds st key n = 
+let enc_rounds st key = 
     let h0 = ST.get() in
-    loop_nospec #h0 n st 
+    loop_nospec #h0 (size 9) st 
       (fun i -> aes_enc st (sub key i (size 1)))
 
 
 inline_for_extraction
-val block_cipher: st:state -> key:keyex -> n:size_t -> ST unit
+val block_cipher: st:state -> key:keyex -> ST unit
 	     (requires (fun h -> live h st /\ live h key))
 	     (ensures (fun h0 _ h1 -> live h1 st /\ live h1 key /\ modifies (loc_buffer st) h0 h1))
-let block_cipher st key n = 
+let block_cipher st key = 
     let k0 = sub key (size 0) (size 1) in
     let kr = sub key (size 1) (size 9) in
     let kn = sub key (size 10) (size 1) in
     add_round_key st k0;
-    enc_rounds st kr (n -. size 1);
+    enc_rounds st kr;
     aes_enc_last st kn
    
+let rcon =  gcreateL [u8(0x8d); u8(0x01); u8(0x02); u8(0x04); u8(0x08); u8(0x10); u8(0x20); u8(0x40); u8(0x80); u8(0x1b); u8(0x36)]
+
+inline_for_extraction
+val aes_keygen_assist: ok:key1 -> ik:key1 -> rcon:uint8 -> ST unit
+			     (requires (fun h -> live h ok /\ live h ik))
+			     (ensures (fun h0 _ h1 -> live h1 ok /\ live h1 ik /\ modifies (loc_buffer ok) h0 h1))
+let aes_keygen_assist ok ik rcon = 
+    ok.(size 0) <- ni_aes_keygen_assist ik.(size 0) rcon		      
+
 inline_for_extraction 
 val key_expansion_step: next:key1 -> prev:key1 -> ST unit
 			     (requires (fun h -> live h prev /\ live h next))
@@ -97,27 +99,13 @@ let key_expansion_step next prev =
     next.(size 0) <- vec128_xor next.(size 0) key
 
 
-inline_for_extraction 
-val key_expansion_step2: next:key1 -> prev:key1 -> ST unit
-			     (requires (fun h -> live h prev /\ live h next))
-			     (ensures (fun h0 _ h1 -> live h1 prev /\ live h1 next /\ modifies (loc_buffer next) h0 h1))
-let key_expansion_step2 next prev = 
-    next.(size 0) <- vec128_shuffle32 next.(size 0) (vec128_shuffle32_spec (u8 2) (u8 2) (u8 2) (u8 2));
-    let key = prev.(size 0) in
-    let key = vec128_xor key (vec128_shift_left key (size 32)) in
-    let key = vec128_xor key (vec128_shift_left key (size 32)) in
-    let key = vec128_xor key (vec128_shift_left key (size 32)) in
-    next.(size 0) <- vec128_xor next.(size 0) key
-
-
-val key_expansion128: keyx:keyex -> key:skey -> ST unit
+val key_expansion: keyx:keyex -> key:skey -> ST unit
 			     (requires (fun h -> live h keyx /\ live h key))
 			     (ensures (fun h0 _ h1 -> live h1 keyx /\ live h1 key /\ modifies (loc_buffer keyx) h0 h1))
-let key_expansion128 keyx key = 
+let key_expansion keyx key = 
     keyx.(size 0) <- vec128_load_le key;
     let h0 = ST.get() in
     (* I WOULD LIKE TO HAVE A LOOP HERE BUT AES_KEYGEN_ASSIST INSISTS ON AN IMMEDIATE RCON *)
-    (* MAYBE WE SHOULD UNROLL ONLY THIS LOOP *)
     (* loop_nospec #h0 (size 10) keyx 
     (fun i -> 
        let prev = sub keyx i (size 1) in
@@ -167,76 +155,11 @@ let key_expansion128 keyx key =
        key_expansion_step next prev
        
 
-val key_expansion256: keyx:keyex -> key:skey256 -> ST unit
-			     (requires (fun h -> live h keyx /\ live h key))
-			     (ensures (fun h0 _ h1 -> live h1 keyx /\ live h1 key /\ modifies (loc_buffer keyx) h0 h1))
-let key_expansion256 keyx key = 
-    keyx.(size 0) <- vec128_load_le (sub key (size 0) (size 16));
-    keyx.(size 1) <- vec128_load_le (sub key (size 16) (size 16));
-    let h0 = ST.get() in
-    (* I WOULD LIKE TO HAVE A LOOP HERE BUT AES_KEYGEN_ASSIST INSISTS ON AN IMMEDIATE RCON *)
-    (* MAYBE WE SHOULD UNROLL ONLY THIS LOOP *)
-       let prev0 = sub keyx (size 0) (size 1) in
-       let prev1 = sub keyx (size 1) (size 1) in
-       let next0 = sub keyx (size 2) (size 1) in
-       let next1 = sub keyx (size 3) (size 1) in
-       aes_keygen_assist next0 prev1 (u8 0x01);
-       key_expansion_step next0 prev0;
-       aes_keygen_assist next1 next0 (u8 0x00);
-       key_expansion_step2 next1 prev1;
-       let prev0 = next0 in
-       let prev1 = next1 in
-       let next0 = sub keyx (size 4) (size 1) in
-       let next1 = sub keyx (size 5) (size 1) in
-       aes_keygen_assist next0 prev1 (u8 0x02);
-       key_expansion_step next0 prev0;
-       aes_keygen_assist next1 next0 (u8 0x00);
-       key_expansion_step2 next1 prev1;
-       let prev0 = next0 in
-       let prev1 = next1 in
-       let next0 = sub keyx (size 6) (size 1) in
-       let next1 = sub keyx (size 7) (size 1) in
-       aes_keygen_assist next0 prev1 (u8 0x04);
-       key_expansion_step next0 prev0;
-       aes_keygen_assist next1 next0 (u8 0x00);
-       key_expansion_step2 next1 prev1;
-       let prev0 = next0 in
-       let prev1 = next1 in
-       let next0 = sub keyx (size 8) (size 1) in
-       let next1 = sub keyx (size 9) (size 1) in
-       aes_keygen_assist next0 prev1 (u8 0x08);
-       key_expansion_step next0 prev0;
-       aes_keygen_assist next1 next0 (u8 0x00);
-       key_expansion_step2 next1 prev1;
-       let prev0 = next0 in
-       let prev1 = next1 in
-       let next0 = sub keyx (size 10) (size 1) in
-       let next1 = sub keyx (size 11) (size 1) in
-       aes_keygen_assist next0 prev1 (u8 0x10);
-       key_expansion_step next0 prev0;
-       aes_keygen_assist next1 next0 (u8 0x00);
-       key_expansion_step2 next1 prev1;
-       let prev0 = next0 in
-       let prev1 = next1 in
-       let next0 = sub keyx (size 12) (size 1) in
-       let next1 = sub keyx (size 13) (size 1) in
-       aes_keygen_assist next0 prev1 (u8 0x20);
-       key_expansion_step next0 prev0;
-       aes_keygen_assist next1 next0 (u8 0x00);
-       key_expansion_step2 next1 prev1;
-       let prev0 = next0 in
-       let prev1 = next1 in
-       let next0 = sub keyx (size 14) (size 1) in
-       aes_keygen_assist next0 prev1 (u8 0x40);
-       key_expansion_step next0 prev0
-    
-       
-
 inline_for_extraction
-val aes_block: st:state -> keyx:keyex -> nonce:state -> counter:size_t -> rounds:size_t -> ST unit
+val aes128_block: st:state -> keyx:keyex -> nonce:state -> counter:size_t -> ST unit
 			     (requires (fun h -> live h st /\ live h keyx /\ live h nonce))
 			     (ensures (fun h0 _ h1 -> live h1 st /\ live h1 nonce /\ live h1 keyx /\ modifies (loc_buffer st) h0 h1))
-let aes_block st keyx nonce counter rounds = 
+let aes128_block st keyx nonce counter = 
     let counter0 = htobe32 (size_to_uint32 counter) in
     let counter1 = htobe32 (size_to_uint32 (counter +. size 1)) in
     let counter2 = htobe32 (size_to_uint32 (counter +. size 2)) in
@@ -245,14 +168,14 @@ let aes_block st keyx nonce counter rounds =
     st.(size 1) <- vec128_insert32 nonce.(size 0) counter1 (u8 3);
     st.(size 2) <- vec128_insert32 nonce.(size 0) counter2 (u8 3);
     st.(size 3) <- vec128_insert32 nonce.(size 0) counter3 (u8 3);
-    block_cipher st keyx rounds
+    block_cipher st keyx
 
 inline_for_extraction noextract
-val aes_alloc: rounds:size_t -> StackInline (keyex * key1)
+val aes128_alloc: unit -> StackInline (keyex * key1)
 			     (requires (fun h -> True))
 			     (ensures (fun h0 (x,y) h1 -> live h1 x /\ live h1 y))
-let aes_alloc rounds = 
-  let keyex = alloca vec128_zero 15ul in
+let aes128_alloc () = 
+  let keyex = alloca vec128_zero 11ul in
   let nonce = alloca vec128_zero 1ul in
   (keyex,nonce)
 
@@ -261,32 +184,20 @@ val aes128_init: keyx:keyex -> nvec:key1 -> key:skey -> nonce:lbytes 12 -> ST un
 			     (ensures (fun h0 b h1 -> modifies (loc_union (loc_buffer keyx) (loc_buffer nvec)) h0 h1))
 let aes128_init keyx (nvec:key1) key nonce = 
   push_frame();
-  key_expansion128 keyx key ; 
+  key_expansion keyx key;
   let nb = alloca 0uy 16ul in
   blit nonce (size 0) nb (size 0) (size 12);
   nvec.(size 0) <- vec128_load_le nb;
   pop_frame()
 
 
-val aes256_init: keyx:keyex -> nvec:key1 -> key:skey -> nonce:lbytes 12 -> ST unit
-			     (requires (fun h -> live h keyx /\ live h nonce /\ live h nvec /\ live h key))
-			     (ensures (fun h0 b h1 -> modifies (loc_union (loc_buffer keyx) (loc_buffer nvec)) h0 h1))
-let aes256_init keyx (nvec:key1) key nonce = 
-  push_frame();
-  key_expansion256 keyx key ; 
-  let nb = alloca 0uy 16ul in
-  blit nonce (size 0) nb (size 0) (size 12);
-  nvec.(size 0) <- vec128_load_le nb;
-  pop_frame()
-
-
-val aes_update4: out:lbytes 64 -> inp:lbytes 64 -> keyx:keyex -> nvec:key1 -> counter:size_t -> rounds:size_t -> ST unit
+val aes128_update4: out:lbytes 64 -> inp:lbytes 64 -> keyx:keyex -> nvec:key1 -> counter:size_t -> ST unit
 			     (requires (fun h -> live h out /\ live h inp /\ live h keyx /\ live h nvec))
 			     (ensures (fun h0 b h1 -> modifies (loc_buffer out) h0 h1))
-let aes_update4 out inp keyx nvec ctr rounds =
+let aes128_update4 out inp keyx nvec ctr =
   push_frame();
   let st = alloca vec128_zero 4ul in
-  aes_block st keyx nvec ctr rounds;
+  aes128_block st keyx nvec ctr;
   st.(size 0) <- vec128_xor st.(size 0) (vec128_load_le (sub inp (size 0) (size 16)));
   st.(size 1) <- vec128_xor st.(size 1) (vec128_load_le (sub inp (size 16) (size 16)));
   st.(size 2) <- vec128_xor st.(size 2) (vec128_load_le (sub inp (size 32) (size 16)));
@@ -297,11 +208,13 @@ let aes_update4 out inp keyx nvec ctr rounds =
   vec128_store_le (sub out (size 48) (size 16)) st.(size 3);
   pop_frame()
 
-val aes_ctr: out:bytes -> inp:bytes -> len:size_t -> keyx:keyex -> nvec:key1 -> counter:size_t -> ST unit
-			     (requires (fun h -> live h out /\ live h inp /\ live h keyx /\ live h nvec))
+val aes128_ctr: out:bytes -> inp:bytes -> len:size_t -> key:skey -> nonce:lbytes 12 -> counter:size_t -> ST unit
+			     (requires (fun h -> live h out /\ live h inp /\ live h key /\ live h nonce))
 			     (ensures (fun h0 _ h1 -> modifies (loc_buffer out) h0 h1))
-let aes_ctr out inp len kex nvec counter = 
+let aes128_ctr out inp len key nonce counter = 
   push_frame();
+  let (kex,nvec) = aes128_alloc () in
+  aes128_init kex nvec key nonce;
   let blocks64 = len /. size 64 in
   let h0 = ST.get() in
   loop_nospec #h0 blocks64 out 
@@ -309,7 +222,7 @@ let aes_ctr out inp len kex nvec counter =
       let ctr = counter +. (i *. size 4) in
       let ib = sub inp (i *. size 64) (size 64) in
       let ob = sub out (i *. size 64) (size 64) in
-      aes_update4 ob ib kex nvec ctr (size 10));
+      aes128_update4 ob ib kex nvec ctr);
   let rem = len %. size 64 in
   if (rem >. size 0) then (
       let ctr = counter +. (blocks64 *. size 4) in
@@ -317,26 +230,9 @@ let aes_ctr out inp len kex nvec counter =
       let ob = sub out (blocks64 *. size 64) rem in
       let last = alloca 0uy 64ul in
       blit ib (size 0) last (size 0) rem;
-      aes_update4 last last kex nvec ctr (size 10);
+      aes128_update4 last last kex nvec ctr;
       blit last (size 0) ob (size 0) rem);
   pop_frame()
 
-let aes128_ctr_encrypt out inp in_len k n c = 
-  push_frame();
-  let (kex,nvec) = aes_alloc (size 10) in
-  aes128_init kex nvec k n;
-  aes_ctr out inp in_len kex nvec c;
-  pop_frame()
-
-let aes128_ctr_decrypt out inp in_len k n c = 
-  aes128_ctr_encrypt out inp in_len k n c
-
-let aes256_ctr_encrypt out inp in_len k n c = 
-  push_frame();
-  let (kex,nvec) = aes_alloc (size 14) in
-  aes256_init kex nvec k n;
-  aes_ctr out inp in_len kex nvec c;
-  pop_frame()
-
-let aes256_ctr_decrypt out inp in_len k n c = 
-  aes128_ctr_encrypt out inp in_len k n c
+let aes128_encrypt out inp in_len k n c = aes128_ctr out inp in_len k n c
+let aes128_decrypt out inp in_len k n c = aes128_ctr out inp in_len k n c
